low/InvariantProofs.v
@@ -1,0 +1,18 @@
+(** Invariants.
+  Contains the proofs of some invariants respected by the functions
+  defined in Rcore, Rinit, and Rfeatures. **)
+
+Require Import Rcore Rfeatures Rinit.
+Require Export Invariants.
+
+
+(* TODO *)
+
+(* I think that it would be easy to use tactics to check that [setup_Rmainloop]
+  is indeed of the form [result_success S globals] or something like that. *)
+
+(** It would be nice to prove that the read-eval-print-loop can not
+  return a [result_impossible]. **)
+
+(** If runs returns a result, then adding fuel does not change it. **)
+
